@prefix rdf:   <http://www.w3.org/1999/02/22-rdf-syntax-ns#> .
@prefix owl: <http://www.w3.org/2002/07/owl#> .
@prefix rdfs: <http://www.w3.org/2000/01/rdf-schema#> .
@prefix xsd: <http://www.w3.org/2001/XMLSchema#> .
@prefix dcat: <http://www.w3.org/ns/dcat#> .
@prefix ids: <https://w3id.org/idsa/core/> .
@prefix idsc: <https://w3id.org/idsa/code/> .
@prefix idsm: <https://w3id.org/idsa/metamodel/> .

# Classes
# -------

ids:ConfigurationModel
    a owl:Class;
    rdfs:label "Configuration Model." @en ;
    rdfs:comment "A Model to represent a Connector's configuration." @en ;
    .

ids:ConnectorMode
    a owl:Class;
    rdfs:label "Connector Mode" @en;
    rdfs:comment "Connector Mode class." @en;
    .


ids:ConnectorStatus
    a owl:Class;
    rdfs:label "Connector Status" @en;
    rdfs:comment "Connector Status class." @en;
    .
    

# Properties
# ----------

ids:connectorDeployMode
    a owl:ObjectProperty;
    rdfs:label "connector Deploy Mode"@en;
    rdfs:domain ids:ConfigurationModel;
    rdfs:range ids:ConnectorMode;
    rdfs:comment "Deploy mode of a Connector, e.g., test deployment vs. productive deployment."@en.

# TODO: necessary? 
ids:connectorStatus
    a owl:ObjectProperty;
    rdfs:label "connector Status"@en;
    rdfs:domain ids:ConfigurationModel;
    rdfs:range ids:ConnectorStatus;
    rdfs:comment "Status of the connector. Possible values include online/ offline/ bad_configuration. "@en.

ids:connectorProxy
    a owl:ObjectProperty;
    rdfs:label "connector Status"@en;
    rdfs:domain ids:ConfigurationModel;
    rdfs:range ids:Proxy;
    rdfs:comment "Status of the connector. Possible values include online/ offline/ bad_configuration. "@en.

# Connector Mode Instances
# ------------------------

idsc:TEST_DEPLOYMENT
    a ids:ConnectorMode;
    rdfs:label "Test Deployment" @en. 
    
idsc:PRODUCTIVE_DEPLOYMENT
    a ids:ConnectorMode;
    rdfs:label "Productive Deployment" @en. 

# Connector Status Instances
# --------------------------

idsc:CONNECTOR_ONLINE
    a ids:ConnectorStatus;
    rdfs:label "Connector Online" @en.

idsc:CONNECTOR_OFFLINE
    a ids:ConnectorStatus;
    rdfs:label "Connector Offline" @en.
    
idsc:CONNECTOR_BAD_CONFIGURED
    a ids:ConnectorStatus;
    rdfs:label "Connector Bad Configured" @en.